CRC32 WIP.

code/c/Yazi_CRC32Table_Codegen.c
@@ -6,11 +6,27 @@ int main(int argc, const char **argv) {
   uint32_t table[4][256];
   gen_crc32_table(table[0], table[1], table[2], table[3]);
 
-  for (int i = 0; i < 1; i++) {
-    for (int j = 0; j < 256; j++) { 
-      printf("0x%.8x ", table[i][j]);
+  printf("uint32_t crc32_table[4][256] = {\n");
+  
+  for (int i = 0; i < 4; i++) {
+    if (i == 0) {
+      printf("  {");
+    } else {
+      printf("{");
+    }
+    for (int j = 0; j < 256; j++) {
+      if (j % 5 == 0) {
+	printf("\n    ");
+      }
+      printf("0x%.8xUL, ", table[i][j]);
+    }
+    printf("\n  }");
+    if (i != 3) {
+      printf(", ");
     }
   }
+  
+  printf("\n};\n");
   
   return 0;
 }
