code/Yazi.CRC32Table.fst
@@ -14,67 +14,7 @@ open FStar.Tactics
 open LowStar.BufferOps
 open Spec.CRC32
 
-let rec logand_mask_aux (a: nat{a > 0}) (n: nat{n >= a}): Lemma
-  (requires (pow2 a) - 1 < pow2 n)
-  (ensures forall i. 
-    (i >= n - a ==> UInt.nth #n ((pow2 a) - 1) i == true) /\
-    (i < n - a ==> UInt.nth #n ((pow2 a) - 1) i == false)) =
-  if n = a then
-    ()
-  else begin
-    Math.Lemmas.pow2_le_compat (n - 1) a;
-    logand_mask_aux a (n - 1)
-  end
-
 #set-options "--z3rlimit 120 --z3seed 1"
-let large_table_val_aux
-  (i: U32.t{U32.v i < 256}) (nzeros: nat{nzeros > 0}) (p p' p'': U32.t): Lemma
-  (requires
-    poly_mod_u32 nzeros i == UInt.to_vec (U32.v p) /\
-    poly_mod_u32 8 (U32.logand p 0xFFul) == UInt.to_vec (U32.v p') /\
-    p'' == U32.shift_right p 8ul)
-  (ensures poly_mod_correct (nzeros + 8) i (U32.logxor p' p'')) =
-   let open U32 in
-   let vi = UInt.to_vec (v i) in
-   let vp = UInt.to_vec (v p) in
-   let vp' = UInt.to_vec (v p') in
-   let vp'' = UInt.to_vec (v p'') in
-   let vpand = UInt.to_vec (U32.v (U32.logand p 0xFFul)) in
-   logand_mask_aux 8 32;
-   assert(forall i.
-     i < 32 - 8 ==> Seq.index vpand i == false /\
-     i >= 32 - 8 ==> Seq.index vpand i == Seq.index vp i);
-   assert(vp' == poly_mod (zero_vec_l 8 vpand));
-
-   assert(forall i.
-     i >= 8 ==> Seq.index vp'' i == Seq.index vp (i - 8) /\
-     i < 8 ==> Seq.index vp'' i == false);
-   poly_mod_zero_suffix vp'' 8;
-   assert(vp'' == poly_mod (zero_vec_r 8 vp''));
-
-   assert(forall i. {:pattern Seq.index (zero_vec_l 8 vpand) i}
-     (i >= 40 - 8 ==> Seq.index (zero_vec_l 8 vpand) i == Seq.index vp (i - 8)) /\
-     (i < 40 - 8 ==> Seq.index (zero_vec_l 8 vpand) i == false));
-
-   assert(forall i. {:pattern Seq.index (zero_vec_r 8 vp'') i}
-     (i < 8 \/ i >= 32 ==> Seq.index (zero_vec_r 8 vp'') i == false) /\
-     (i >= 8 /\ i < 32 ==> Seq.index (zero_vec_r 8 vp'') i == Seq.index vp (i - 8)));
-
-   let sum = (zero_vec_l 8 vpand) +@ (zero_vec_r 8 vp'') in
-   assert(forall i. {:pattern Seq.index sum i}
-     (i < 8 ==> Seq.index sum i == false) /\
-     (i >= 8 ==> Seq.index sum i == Seq.index vp (i - 8)));
-   assert(Seq.equal sum (zero_vec_l 8 vp));
-   
-   poly_mod_add (zero_vec_l 8 vpand) (zero_vec_r 8 vp'');
-   assert(poly_mod sum == poly_mod (zero_vec_l 8 vp));
-
-   assert(vp' +@ vp'' == poly_mod (zero_vec_l 8 (poly_mod (zero_vec_l nzeros vi))));
-   poly_mod_zero_prefix (zero_vec_l nzeros vi) 8;
-   assert(vp' +@ vp'' == poly_mod (zero_vec_l 8 (zero_vec_l nzeros vi)));
-   zero_vec_l_app vi nzeros 8;
-   assert(vp' +@ vp'' == poly_mod (zero_vec_l (nzeros + 8) vi))
-
 let rec uint_one_vec (#n: nat{n > 0}) (v: UInt.uint_t n): Lemma
   (requires v == 1)
   (ensures forall i. {:pattern UInt.nth v i}
@@ -99,7 +39,6 @@ let mask_logor_status (#n: nat{n > 0}) (s: nat{s < n}) (mask v: UInt.uint_t n): 
     (j == n - 1 - s ==> UInt.nth (UInt.logor v mask) j == true)) =
   mask_bit_status s mask
 
-#set-options "--z3rlimit 120 --z3seed 1"
 inline_for_extraction
 private let poly_mask (i: U32.t{(U32.v i) < 32}) (p: U32.t{
   let p' = U32.v p in
