specs/Spec.CRC32.Bits.fst
@@ -1,7 +1,10 @@
 module Spec.CRC32.Bits
 
 module BV = FStar.BitVector
+module Math = FStar.Math.Lemmas
 module Seq = FStar.Seq
+module U32 = FStar.UInt32
+module UInt = FStar.UInt
 
 #set-options "--z3rlimit 200 --z3seed 1"
 let poly_xor_zero_prefix (#n: nat{n >= 32}) (a: BV.bv_t n) (m: nat{m > 0}): Lemma
@@ -250,3 +253,121 @@ let rec poly_mod_zero_suffix a m =
       poly_mod (zero_vec_r (m - 1) a);
     };
     poly_mod_zero_suffix a (m - 1)
+
+private let rec logand_mask_aux (a: nat{a > 0}) (n: nat{n >= a}): Lemma
+  (requires (pow2 a) - 1 < pow2 n)
+  (ensures forall i. 
+    (i >= n - a ==> UInt.nth #n ((pow2 a) - 1) i == true) /\
+    (i < n - a ==> UInt.nth #n ((pow2 a) - 1) i == false)) =
+  if n = a then
+    ()
+  else begin
+    Math.Lemmas.pow2_le_compat (n - 1) a;
+    logand_mask_aux a (n - 1)
+  end
+
+let large_table_val_aux i nzeros p p' p'' =
+   let open U32 in
+   let vi = UInt.to_vec (v i) in
+   let vp = UInt.to_vec (v p) in
+   let vp' = UInt.to_vec (v p') in
+   let vp'' = UInt.to_vec (v p'') in
+   let vpand = UInt.to_vec (U32.v (U32.logand p 0xFFul)) in
+   logand_mask_aux 8 32;
+   assert(forall i.
+     i < 32 - 8 ==> Seq.index vpand i == false /\
+     i >= 32 - 8 ==> Seq.index vpand i == Seq.index vp i);
+   assert(vp' == poly_mod (zero_vec_l 8 vpand));
+
+   assert(forall i.
+     i >= 8 ==> Seq.index vp'' i == Seq.index vp (i - 8) /\
+     i < 8 ==> Seq.index vp'' i == false);
+   poly_mod_zero_suffix vp'' 8;
+   assert(vp'' == poly_mod (zero_vec_r 8 vp''));
+
+   assert(forall i. {:pattern Seq.index (zero_vec_l 8 vpand) i}
+     (i >= 40 - 8 ==> Seq.index (zero_vec_l 8 vpand) i == Seq.index vp (i - 8)) /\
+     (i < 40 - 8 ==> Seq.index (zero_vec_l 8 vpand) i == false));
+
+   assert(forall i. {:pattern Seq.index (zero_vec_r 8 vp'') i}
+     (i < 8 \/ i >= 32 ==> Seq.index (zero_vec_r 8 vp'') i == false) /\
+     (i >= 8 /\ i < 32 ==> Seq.index (zero_vec_r 8 vp'') i == Seq.index vp (i - 8)));
+
+   let sum = (zero_vec_l 8 vpand) +@ (zero_vec_r 8 vp'') in
+   assert(forall i. {:pattern Seq.index sum i}
+     (i < 8 ==> Seq.index sum i == false) /\
+     (i >= 8 ==> Seq.index sum i == Seq.index vp (i - 8)));
+   assert(Seq.equal sum (zero_vec_l 8 vp));
+   
+   poly_mod_add (zero_vec_l 8 vpand) (zero_vec_r 8 vp'');
+   assert(poly_mod sum == poly_mod (zero_vec_l 8 vp));
+
+   assert(vp' +@ vp'' == poly_mod (zero_vec_l 8 (poly_mod (zero_vec_l nzeros vi))));
+   poly_mod_zero_prefix (zero_vec_l nzeros vi) 8;
+   assert(vp' +@ vp'' == poly_mod (zero_vec_l 8 (zero_vec_l nzeros vi)));
+   zero_vec_l_app vi nzeros 8;
+   assert(vp' +@ vp'' == poly_mod (zero_vec_l (nzeros + 8) vi))
+
+open FStar.Seq
+  
+let rec crc32_u8_to_bits_append #m1 #m2 #n s1 s2 buf =
+  match m1 with
+  | 0 -> assert(Seq.equal (Seq.append s1 s2) s2)
+  | _ ->
+    let l = if m1 > 0 then
+      if n = 0 then 32 + 8 * m1 else n + 8 * m1
+    else
+      n
+    in
+    if m2 = 0 then begin
+      assert(Seq.equal (s1 @| s2) s1);
+      assert(
+        (normalize_term (crc32_u8_to_bits #m2 #l s2 (crc32_u8_to_bits #m1 #n s1 buf))) ==
+        crc32_u8_to_bits #m1 #n s1 buf)
+    end else if m1 = 1 then
+      calc (==) {
+        crc32_u8_to_bits #m2 #l s2 (crc32_u8_to_bits #m1 #n s1 buf);
+        =={}
+        crc32_u8_to_bits #m2 #l s2 (crc32_append_8bit buf (Seq.head s1));
+        =={Seq.lemma_head_append s1 s2}
+        crc32_u8_to_bits #m2 #l s2 (crc32_append_8bit buf (Seq.head (s1 @| s2)));
+        =={
+          Seq.lemma_tail_append s1 s2;
+          assert(Seq.equal (Seq.tail (s1 @| s2)) s2)
+        }
+        crc32_u8_to_bits #m2 #l (Seq.tail (s1 @| s2)) (crc32_append_8bit buf (Seq.head (s1 @| s2)));
+        =={assert(1 + m2 > 1)}
+        crc32_u8_to_bits #(1 + m2) #n (s1 @| s2) buf;
+      }
+    else
+      calc (==) {
+        crc32_u8_to_bits #m2 #l s2 (crc32_u8_to_bits #m1 #n s1 buf);
+        =={}
+        crc32_u8_to_bits #m2 #l s2 (crc32_u8_to_bits
+          #(m1 - 1) #_
+          (Seq.tail s1)
+          (crc32_append_8bit buf (Seq.head s1)));
+        =={
+          crc32_u8_to_bits_append
+            #(m1 - 1)
+            #m2
+            #(if n = 0 then 40 else n + 8)
+            (Seq.tail s1)
+            s2
+            (crc32_append_8bit buf (Seq.head s1))
+        }
+        crc32_u8_to_bits
+          #(m1 + m2 - 1) #_
+          ((Seq.tail s1) @| s2) 
+          (crc32_append_8bit buf (Seq.head s1));
+        =={
+          Seq.lemma_tail_append s1 s2;
+          Seq.lemma_head_append s1 s2
+        }
+        crc32_u8_to_bits
+          #(m1 + m2 - 1) #_
+          (Seq.tail (s1 @| s2))
+          (crc32_append_8bit buf (Seq.head (s1 @| s2)));
+        =={}
+        crc32_u8_to_bits #(m1 + m2) #n (s1 @| s2) buf;
+      }
