specs/Spec.CRC32.Bits.fsti
@@ -1,8 +1,16 @@
 module Spec.CRC32.Bits
+
+module B = LowStar.Buffer
+module CB = LowStar.ConstBuffer
 module BV = FStar.BitVector
+module HS = FStar.HyperStack
+module Math = FStar.Math.Lib
 module Seq = FStar.Seq
+module U8 = FStar.UInt8
 module U32 = FStar.UInt32
 module UInt = FStar.UInt
+
+open FStar.Mul
 
 unfold let zero_vec_l (#n: nat{n > 0}) (m: nat) (a: BV.bv_t n): Tot (res: BV.bv_t (n + m){
   forall i.
@@ -99,7 +107,7 @@ let rec poly_mod (#n: nat{n > 32}) (a: BV.bv_t n): Tot (BV.bv_t 32) =
 val poly_mod_zero: #n: nat{n > 32} -> a: BV.bv_t n {a == BV.zero_vec #n} -> Lemma
   (ensures poly_mod a == BV.zero_vec #32)
 
-val poly_mod_add: #n: nat{n > 32} -> a: BV.bv_t n ->  b: BV.bv_t n -> Lemma
+val poly_mod_add: #n: nat{n > 32} -> a: BV.bv_t n -> b: BV.bv_t n -> Lemma
   (ensures (poly_mod a) +@ (poly_mod b) == poly_mod (a +@ b))
 
 val poly_mod_zero_prefix: #n: nat{n > 32} -> a: BV.bv_t n -> m: nat{m > 0} -> Lemma
@@ -116,9 +124,113 @@ unfold let poly_mod_correct (nzeros: nat{nzeros > 0}) (d res: U32.t) =
 unfold let poly_mod_u32 (nzeros: nat{nzeros > 0}) (d: U32.t) =
   poly_mod (zero_vec_l nzeros (UInt.to_vec (U32.v d)))
 
+val large_table_val_aux:
+    i: U32.t{U32.v i < 256}
+  -> nzeros: nat{nzeros > 0}
+  -> p: U32.t
+  -> p': U32.t
+  -> p'': U32.t
+  -> Lemma
+  (requires
+    poly_mod_u32 nzeros i == UInt.to_vec (U32.v p) /\
+    poly_mod_u32 8 (U32.logand p 0xFFul) == UInt.to_vec (U32.v p') /\
+    p'' == U32.shift_right p 8ul)
+  (ensures poly_mod_correct (nzeros + 8) i (U32.logxor p' p''))
+
 let poly_mod_correct_eq (nzeros: nat{nzeros > 0}) (d res: U32.t): Lemma
   (requires poly_mod_correct nzeros d res)
   (ensures poly_mod_u32 nzeros d == UInt.to_vec (U32.v res)) =
   let open U32 in
   assert(forall i. UInt.nth (v res) i == Seq.index (UInt.to_vec (v res)) i);
   assert(Seq.equal (poly_mod (zero_vec_l nzeros (UInt.to_vec (U32.v d)))) (UInt.to_vec (v res)))
+
+type table_buf = buf: B.buffer U32.t{B.length buf == 256}
+
+let sub_table_correct
+  (j: nat{j <= 256})
+  (nzeros: nat{nzeros > 0})
+  (h: HS.mem)
+  (buf: table_buf) =
+  (B.live h buf) /\
+  (forall i. i < j ==>
+  poly_mod_correct nzeros (U32.uint_to_t i) (Seq.index (B.as_seq h buf) i))
+
+let table_correct
+  (nzeros: nat{nzeros > 0})
+  (h: HS.mem)
+  (buf: B.buffer U32.t{B.length buf == 256}) = sub_table_correct (B.length buf) nzeros h buf
+
+private let rec seq_append_index_l (#t: Type) (a b: Seq.seq t): Lemma
+  (ensures forall i. i < Seq.length a ==> Seq.index a i == Seq.index (Seq.append a b) i)
+  (decreases Seq.length a) =
+  match Seq.length a with
+  | 0 -> ()
+  | _ -> seq_append_index_l (Seq.tail a) b
+
+private let bit_padding (#len: nat) (buf: Seq.seq U8.t{Seq.length buf == len}):
+  Tot (res: Seq.seq U8.t{
+    (Seq.length res == len + 4) /\
+    (forall i.
+      (i < 4 ==> Seq.index res i == 0uy) /\
+      (i >= 4 ==> Seq.index res i = Seq.index buf (i - 4)))
+  }) =
+  let pad = Seq.create 4 0uy in
+  let r = Seq.append pad buf in
+  seq_append_index_l pad buf;
+  r
+
+type crc32_buf_len = n: nat{n == 0 \/ n > 32}
+
+let crc32_append_8bit (#n: crc32_buf_len) (buf: BV.bv_t n) (b: U8.t):
+  Tot (BV.bv_t (if n = 0 then 40 else n + 8)) =
+  let v' = UInt.to_vec (U8.v b) in
+  let open Seq in
+  if n = 0 then
+    zero_vec_l 8 (gf2_plus (BV.ones_vec #32) (BV.zero_vec #24 @| v'))
+  else
+    let padding = (BV.zero_vec #24) @| v' @| (BV.zero_vec #(n - 32)) in
+    zero_vec_l 8 (buf +@ padding)
+
+let rec crc32_u8_to_bits
+  (#m: nat)
+  (#n: crc32_buf_len)
+  (data: Seq.seq U8.t {Seq.length data == m})
+  (buf: BV.bv_t n):
+  Tot (BV.bv_t (if m > 0 then
+    if n = 0 then 32 + 8 * m else n + 8 * m
+  else
+    n))
+  (decreases m) =
+  if m > 1 then
+    crc32_u8_to_bits
+      #(m - 1)
+      #_
+      (Seq.tail data)
+      (crc32_append_8bit buf (Seq.head data))
+  else if m = 1 then
+    crc32_append_8bit buf (Seq.head data)
+  else
+    buf
+
+#set-options "--z3rlimit 120 --z3seed 1"
+val crc32_u8_to_bits_append:
+    #m1: nat
+  -> #m2: nat
+  -> #n: crc32_buf_len
+  -> s1: Seq.seq U8.t{Seq.length s1 == m1}
+  -> s2: Seq.seq U8.t{Seq.length s2 == m2}
+  -> buf: BV.bv_t n
+  -> Lemma (ensures
+    crc32_u8_to_bits #m2 #(if m1 > 0 then
+      if n = 0 then 32 + 8 * m1 else n + 8 * m1
+    else
+      n) s2 (crc32_u8_to_bits #m1 #n s1 buf) ==
+    crc32_u8_to_bits #(m1 + m2) #n (Seq.append s1 s2) buf)
+
+private unfold let crc32_to_vec (v: U32.t) =
+  UInt.to_vec (UInt.logxor (U32.v v) ((pow2 32) - 1))
+
+let crc32_matched (#n: crc32_buf_len) (buf: BV.bv_t n) (v: U32.t) (xor: bool) =
+  let v' = if xor then crc32_to_vec v else UInt.to_vec (U32.v v) in
+  (n == 0 ==> v' == (if xor then BV.zero_vec #32 else BV.ones_vec #32)) /\
+  (n > 0 ==> v' == poly_mod buf)
