code/Yazi.CRC32.fst
@@ -1,0 +1,210 @@
+module Yazi.CRC32
+module B = LowStar.Buffer
+module BV = FStar.BitVector
+module Cast = FStar.Int.Cast
+module U32 = FStar.UInt32
+module UInt = FStar.UInt
+
+open FStar.Seq
+open LowStar.BufferOps
+open Spec.CRC32
+    
+#set-options "--z3rlimit 120 --z3seed 1 --fuel 16 --ifuel 16"
+let rec cast_zero_prefix (#n: nat) (v: UInt.uint_t n) (m: nat{m >= n}): Lemma
+  (requires pow2 n <= pow2 m)
+  (ensures UInt.to_vec #m v == (Seq.create (m - n) false) @| (UInt.to_vec v)) =
+  match m - n with
+  | 0 -> assert(Seq.equal (UInt.to_vec #m v) ((Seq.create (m - n) false) @| (UInt.to_vec v)))
+  | _ ->
+    if n >= 1 then
+      calc (==) {
+        UInt.to_vec #m v;
+        =={}
+        (UInt.to_vec #(m - 1) (v / 2)) @| (Seq.create 1 (v % 2 = 1));
+        =={
+          Math.Lemmas.pow2_le_compat (m - 1) (n - 1);
+          assert(v / 2 <= pow2 (n - 1));
+          cast_zero_prefix #(n - 1) (v / 2) (m - 1)
+        }
+        ((Seq.create (m - n) false) @| (UInt.to_vec #(n - 1) (v / 2))) @|
+        (Seq.create 1 (v % 2 = 1));
+        =={
+          Seq.append_assoc
+            (Seq.create (m - n) false)
+            (UInt.to_vec #(n - 1) (v / 2))
+            (Seq.create 1 (v % 2 = 1))
+        }
+        (Seq.create (m - n) false) @|
+        ((UInt.to_vec #(n - 1) (v / 2)) @| (Seq.create 1 (v % 2 = 1)));
+        =={}
+        (Seq.create (m - n) false) @| (UInt.to_vec v);
+      }
+    else begin
+      assert(Seq.equal (UInt.to_vec #m v) (Seq.create m false));
+      assert(UInt.to_vec #n v == Seq.empty #bool);
+      assert(Seq.equal (UInt.to_vec #m v) ((Seq.create m false) @| (Seq.empty #bool)))
+    end
+
+private unfold let u8_padding (b: U8.t) (n: nat{n > 32}): Tot (BV.bv_t n) =
+  (BV.zero_vec #24) @| (UInt.to_vec (U8.v b)) @| (BV.zero_vec #(n - 32))
+
+#set-options "--z3rlimit 120 --z3seed 1"
+let do1_logxor (#m: crc32_buf_len) (prev: BV.bv_t m) (crc: U32.t) (b: U8.t): Lemma
+  (requires crc32_matched #m prev crc false)
+  (ensures
+    (m == 0 ==>
+      UInt.to_vec (U32.v (U32.logxor crc (Cast.uint8_to_uint32 b))) ==
+      (BV.ones_vec #32 +@ (zero_vec_l 24 (UInt.to_vec (U8.v b))))) /\
+    (m > 32 ==>
+      UInt.to_vec (U32.v (U32.logxor crc (Cast.uint8_to_uint32 b))) ==
+      poly_mod (prev +@ (u8_padding b m)))) =
+  let open U32 in
+  let b32 = Cast.uint8_to_uint32 b in
+  let vb32: BV.bv_t 32 = UInt.to_vec (v b32) in
+  let vcrc = UInt.to_vec (v crc) in
+  cast_zero_prefix (U8.v b) 32;
+  if m > 32 then
+    calc (==) {
+      vcrc +@ vb32;
+      =={}
+      (poly_mod prev) +@ vb32;
+      =={poly_mod_zero_suffix vb32 (m - 32)}
+      (poly_mod prev) +@ (poly_mod (zero_vec_r (m - 32) vb32));
+      =={
+        assert(Seq.equal (zero_vec_r (m - 32) vb32) (u8_padding b m))
+      }
+      (poly_mod prev) +@ (poly_mod (u8_padding b m));
+      =={poly_mod_add prev (u8_padding b m)}
+      poly_mod (prev +@ (u8_padding b m));
+    }
+  else
+    ()
+
+#set-options "--z3rlimit 200 --ifuel 128 --fuel 128 --z3seed 1"
+let logand_256 (r: U32.t): Lemma
+  (ensures forall (i: nat{i < 32}).
+    (i < 32 - 8 ==> UInt.nth (U32.v (U32.logand r 0xFFul)) i == false) /\
+    (i >= 32 - 8 ==> UInt.nth (U32.v (U32.logand r 0xFFul)) i == UInt.nth (U32.v r) i)) =
+  let open U32 in
+  let mask = v 0xFFul in
+  assert(forall (i: nat{i < 32}).
+    (i < 32 - 8 ==> UInt.nth mask i == false) /\
+    (i >= 32 - 8 ==> UInt.nth mask i == true));
+  assert(forall (i: nat{i < 32}).
+    (i < 32 - 8 ==> UInt.nth (UInt.logand (v r) (v 0xFFul)) i == false) /\
+    (i >= 32 - 8 ==> UInt.nth (UInt.logand (v r) (v 0xFFul)) i == UInt.nth (U32.v r) i))
+
+#set-options "--z3rlimit 200 --z3seed 1"
+let do1_shift_right_logxor (r: U32.t) (t: U32.t): Lemma
+  (requires poly_mod_correct 8 (U32.logand r 0xFFul) t)
+  (ensures
+     UInt.to_vec (U32.v (U32.logxor (U32.shift_right r 8ul) t)) ==
+     poly_mod (zero_vec_l 8 (UInt.to_vec (U32.v r)))) =
+  let vr = UInt.to_vec (U32.v r) in
+  let r' = U32.shift_right r 8ul in
+  let vr' = UInt.to_vec (U32.v r') in
+  let i = U32.logand r 0xfful in
+  let vi = UInt.to_vec (U32.v i) in
+  poly_mod_correct_eq 8 i t;
+  assert(poly_mod (zero_vec_l 8 vi) == UInt.to_vec (U32.v t));
+  poly_mod_zero_suffix vr' 8;
+  assert(poly_mod (zero_vec_r 8 vr') == vr');
+  poly_mod_add (zero_vec_r 8 vr') (zero_vec_l 8 vi);
+  assert((poly_mod (zero_vec_r 8 vr')) +@ (poly_mod (zero_vec_l 8 vi)) ==
+    poly_mod ((zero_vec_r 8 vr') +@ (zero_vec_l 8 vi)));
+  assert(forall j. {:pattern (Seq.index (zero_vec_r 8 vr') j)}
+    ((j >= 8 /\ j < 40 - 8) ==> Seq.index (zero_vec_r 8 vr') j == Seq.index vr (j - 8)) /\
+    ((j < 8 \/ j >= 40 - 8) ==> Seq.index (zero_vec_r 8 vr') j == false));
+  logand_256 r;
+  assert(forall (j: nat{j < 40}). {:pattern (Seq.index (zero_vec_l 8 vi) j)}
+    (j >= 40 - 8 ==> Seq.index (zero_vec_l 8 vi) j == Seq.index vr (j - 8)) /\
+    (j < 40 - 8  ==> Seq.index (zero_vec_l 8 vi) j == false));
+  assert(Seq.equal
+    ((zero_vec_r 8 vr') +@ (zero_vec_l 8 vi))
+    (zero_vec_l 8 (UInt.to_vec (U32.v r))))
+
+inline_for_extraction
+private let do1
+  (#m: Ghost.erased crc32_buf_len)
+  (t8: Spec.table_buf)
+  (prev: Ghost.erased (BV.bv_t m))
+  (crc: U32.t)
+  (b: U8.t):
+  ST.Stack U32.t
+  (requires fun h -> table_correct 8 h t8 /\ crc32_matched #m prev crc false)
+  (ensures fun h0 res h1 ->
+    let curr = crc32_append_8bit #m prev b in
+    M.modifies M.loc_none h0 h1 /\
+    crc32_matched #(if Ghost.reveal m = 0 then 40 else m + 8) curr res false) =
+  let b' = Cast.uint8_to_uint32 b in
+  let open U32 in
+  let r = crc ^^ b' in 
+  UInt.logand_le (v r) (v 0xFFul);
+  let tv = t8.(r &^ 0xFFul) in
+  let r' = r >>^ 8ul in
+  let p = r' ^^ tv in
+  do1_shift_right_logxor r tv;
+  do1_logxor prev crc b;
+  assert(UInt.to_vec (v p) == poly_mod (zero_vec_l 8 (UInt.to_vec (v r))));
+  if Ghost.reveal m = 0 then begin
+    assert(poly_mod (zero_vec_l 8 (UInt.to_vec (v r))) ==
+      poly_mod (zero_vec_l 8 (BV.ones_vec #32 +@ (zero_vec_l 24 (UInt.to_vec (U8.v b))))));
+    assert(Seq.equal
+      (zero_vec_l 8 (BV.ones_vec #32 +@ (zero_vec_l 24 (UInt.to_vec (U8.v b)))))
+      (crc32_append_8bit prev b))
+  end else begin
+    assert(poly_mod (zero_vec_l 8 (UInt.to_vec (v r))) ==
+      poly_mod (zero_vec_l 8 (poly_mod (prev +@ (u8_padding b m)))));
+    poly_mod_zero_prefix (prev +@ (u8_padding b m)) 8;
+    assert(Seq.equal
+      (zero_vec_l 8 (prev +@ (u8_padding b m)))
+      (crc32_append_8bit prev b))
+  end;
+  p
+
+inline_for_extraction
+private let rec do1_remain
+  (t8: Spec.table_buf)
+  (l: U32.t)
+  (buf: B.buffer U8.t{B.length buf == U32.v l})
+  (m: Ghost.erased nat)
+  (data: Ghost.erased (Seq.seq U8.t){Seq.length data == Ghost.reveal m})
+  (r: U32.t{U32.v r <= (U32.v l) % 4})
+  (crc: U32.t):
+  ST.Stack (U32.t * B.buffer U8.t)
+  (decreases (U32.v r) - ((U32.v l) % 4))
+  (requires fun h ->
+    let curr = crc32_u8_to_bits #m #0 (data @| Seq.slice 0 (B.as_seq h buf) r) crc false in
+    B.live h buf /\
+    table_correct 8 h t8 /\
+    crc32_matched
+      (crc32_u8_to_bits #m #0 data (Seq.empty #bool))
+      crc false)
+  (ensures fun h0 res h1 ->
+    let curr = crc32_u8_to_bits
+      #(m + ((U32.v l) % 4))
+      #0
+      (data @| (Seq.slice (B.as_seq h1 buf) 0 ((U32.v l) % 4)))
+      (Seq.empty #bool) in
+    M.modifies M.loc_none h0 h1 /\
+    crc32_matched #_ curr (fst res) false) =
+  let open U32 in
+  if r <^ (l %^ 4ul) then begin
+    admit();
+    do1_remain t8 l buf m data
+      (r +^ 1ul)
+      (do1
+        t8
+        (crc32_u8_to_bits #m #0 data (Seq.empty #bool))
+        crc
+        (B.index buf r))
+  end else begin
+    (crc, buf)
+  end
+
+let crc32_impl #n prev t8 t16 t24 t32 crc buf len =
+  let open U32 in
+  ST.push_frame ();
+  admit();
+  ST.pop_frame ();
+  0ul
