code/Yazi.CRC32.fsti
@@ -1,0 +1,38 @@
+module Yazi.CRC32
+
+module B = LowStar.Buffer
+module BV = FStar.BitVector
+module Ghost = FStar.Ghost
+module HS = FStar.HyperStack
+module M = LowStar.Modifies
+module U32 = FStar.UInt32
+module U8 = FStar.UInt8
+module Seq = FStar.Seq
+module Spec = Spec.CRC32
+module ST = FStar.HyperStack.ST
+
+private unfold let table_group_correct h t8 t16 t24 t32 =
+  Spec.table_correct 8 h t8 /\
+  Spec.table_correct 16 h t16 /\
+  Spec.table_correct 24 h t24 /\
+  Spec.table_correct 32 h t32
+
+val crc32_impl:
+    #n: Ghost.erased nat{Ghost.reveal n == 0 /\ n > 32}
+  -> prev: Ghost.erased (BV.bv_t n)
+  -> t8: Spec.table_buf
+  -> t16: Spec.table_buf
+  -> t24: Spec.table_buf
+  -> t32: Spec.table_buf
+  -> crc: U32.t
+  -> buf: B.buffer U8.t
+  -> len: U32.t{B.length buf == U32.v len}
+  -> ST.Stack U32.t
+  (requires fun h ->
+    B.live h buf /\
+    table_group_correct h t8 t16 t24 t32 /\
+    Spec.crc32_matched #n prev crc true)
+  (ensures fun h0 res h1 ->
+    M.modifies M.loc_none h0 h1 /\
+    Spec.crc32_matched 
+      (Spec.crc32_append_buf #n #(U32.v len) prev (B.as_seq h1 buf)) res true)
